started fx10

FX10.v
@@ -1,1 +1,73 @@
-(* Featherweight X10 Implementation *)
+(** Featherweight X10 Implementation *)
+
+Definition array := list nat.
+Notation "x :: l" := (cons x l)
+                     (at level 60, right associativity).
+Notation "[ ]" := nil.
+Notation "[ x ; .. ; y ]" := (cons x .. (cons y nil) ..).
+
+Fixpoint access (A : array) (index : nat) : nat :=
+  match index with
+  | O => match A with
+    | nil => O
+    | h :: t => h
+  end
+  | S index' => match A with
+    | nil => O
+    | h :: t => access t index'
+  end
+end.
+
+Example test_access0:  (access [1; 2; 3] 0) = 1.
+Proof. simpl. reflexivity.  Qed.
+Example test_access1:  (access [1; 2; 3] 1) = 2.
+Proof. simpl. reflexivity.  Qed.
+Example test_access2:  (access [1; 2; 3] 2) = 3.
+Proof. simpl. reflexivity.  Qed.
+Example test_access3:  (access [1; 2; 3] 3) = 0.
+Proof. simpl. reflexivity.  Qed.
+
+Fixpoint insert (A : array) (index : nat) (value : nat) : array := 
+  match index with
+  | O => match A with
+    | nil => value :: nil
+    | h :: t => value :: t
+  end
+  | S index' => match A with
+    | nil => value :: nil
+    | h :: t => h :: insert t index' value
+  end
+end.
+
+Example test_insert0:  (insert [1; 1; 1] 0 2) = [2; 1; 1].
+Proof. simpl. reflexivity.  Qed.
+Example test_insert1:  (insert [1; 1; 1] 1 2) = [1; 2; 1].
+Proof. simpl. reflexivity.  Qed.
+Example test_insert2:  (insert [1; 1; 1] 2 2) = [1; 1; 2].
+Proof. simpl. reflexivity.  Qed.
+Example test_insert3:  (insert [1; 1; 1] 3 2) = [1; 1; 1; 2].
+Proof. simpl. reflexivity.  Qed.
+
+
+
+Inductive statement : Type :=
+| skip : statement
+| seq (i : instr) (s : statement) : statement
+.
+
+Definition instr : Type :=
+| skip : instr
+(* a[d] = e *)
+(* while (a[d] != 0) s *)
+| async (s : statement) : instr
+| finish (s : statement) : instr
+| call
+.
+
+Definition expr : Type := 
+| nat : expr
+(* a[d] + 1 *)
+.
+
+
+
